cogent/isa/CogentHelper.thy
@@ -326,7 +326,7 @@ fun kind_proof_single (@{term SomeT} $ t) k ctxt hint = let
     val tac = (case hint of
             (KindingTacs tac) => tac
             | _ => raise ERROR ("kind_proof_single: not a kinding tac"))
-    val t = betapplys (@{term "kinding"}, [k, t, (@{schematic_term "?k :: kind"})])
+    val t = betapplys (@{term "kinding"}, [@{term "0::nat"}, k, @{term "{} :: (ptr_layout \<times> lrepr) set"}, t, (@{schematic_term "?k :: kind"})])
     val ct = Thm.cterm_of ctxt (@{term Trueprop} $ t)
     val rs = EVERY (map (fn t => interpret_tac t ctxt 1) tac) (Thm.trivial ct)
     val t = (case Seq.pull rs of
@@ -346,7 +346,7 @@ fun kind_proofs ((@{term SomeT} $ t) :: ts) k ctxt hints = let
         [RTac thm] => Display.pretty_thm ctxt thm |> Pretty.writeln
       | _ => warning "unexpected kinding tacs"
 *)
-    val t = betapplys (@{term "kinding"}, [k, t, (@{schematic_term "?k :: kind"})])
+    val t = betapplys (@{term "kinding"}, [@{term "0::nat"}, k, @{term "{} :: (ptr_layout \<times> lrepr) set"}, t, (@{schematic_term "?k :: kind"})])
     val ct = Thm.cterm_of ctxt (@{term Trueprop} $ t)
     val rs = EVERY (map (fn t => interpret_tac t ctxt 1) tacs) (Thm.trivial ct)
     val t = (case Seq.pull rs of
